Core/ProgramRules.v
@@ -1,15 +1,17 @@
-(* From LHL.Core Require Import
+From LHL.Core Require Import
   Program
   Specs
   Traces
   Logic
-  LogicFacts.
+  LogicFacts
+  ProgramFacts.
 
 From Coq Require Import
   Program.Equality.
 
+From LHL.Util Require Import
+  Tactics.
 
-Unset Guard Checking.
 Section rules.
 
 Context
@@ -19,61 +21,76 @@ Context
   {VF : Spec F}
   {R G : Relt VE VF}.
 
-Lemma lemNoOp {A P Q} {C : Prog E A} :
-  VerifyProg i R G P C Q ->
+Lemma lemNoOp {A Q} {P : Relt VE VF} {C : Prog E A} :
+  forall QS,
+  Stable R QS ->
+  SilentStep i G P QS ->
+  VerifyProg i R G (P ->> QS) C Q ->
   VerifyProg i R G P (NoOp C) Q.
 intros.
-constructor.
-exact H.
+econstructor. exact H. easy. easy.
 Qed.
 
 Lemma lemRet {A P Q} {v : A} :
-  (forall s ρ t σ, P s ρ -> Q v s ρ t σ) ->
+  (forall v, P ==> Q v) ->
   VerifyProg i R G P (ret v) Q.
 intros.
 constructor.
 unfold sub, subRelt, id.
-intros.
-psimpl.
-apply H.
-easy.
+intros. psimpl.
+apply H. easy.
 Qed.
 
-Lemma lemCall {A P Q S} {m : E A} :
+Lemma lemCall {A Q S} {P : Relt VE VF} {m : E A} :
   Stable R Q ->
   Stable R S ->
   Commit i G P (CallEv m) Q ->
-  (forall v, Commit i G (prComp P id ->> Q) (RetEv m v) (S v)) ->
-  VerifyProg i R G P (call m) (fun v => Q ->> S v).
+  (forall v, Commit i G (P ->> Q) (RetEv m v) (S v)) ->
+  VerifyProg i R G P (call m) (fun v => P ->> Q ->> S v).
 intros.
-econstructor.
-exact H.
-exact H0.
+econstructor. exact H. exact H0.
 unfold Commit, id.
-intros.
-psimpl.
+intros. psimpl.
 apply H1.
-easy.
-easy.
-easy.
-easy.
-split.
-apply H2.
-constructor.
-unfold sub, subRelt, id.
-intros.
-psimpl.
-psplit.
-exact H4.
+exists x, x0.
+easy. easy. easy. easy.
+intros. specialize (H2 v).
+split. easy.
+econstructor. unfold sub, subRelt. intros.
 easy.
 Qed.
 
-Lemma lemBind {A B P Q S} {C : Prog E A} {k : A -> Prog E B} :
-  VerifyProg i R G P C Q ->
-  (forall v, VerifyProg i R G (P <<- Q) (k v) S) ->
-  VerifyProg i R G P (x <- C; k x) (fun v => Q ->> S v).
+Axiom undef:forall{a},a.
+
+CoFixpoint lemBind {A B P Q S} {C : Prog E A} {k : A -> Prog E B}
+  (H : VerifyProg i R G P C Q) :
+  (forall v, VerifyProg i R G (Q v) (k v) S) ->
+  VerifyProg i R G P (x <- C; k x) S.
 intros.
-Admitted.
+destruct H.
+{
+  rewrite frobProgId at 1. simpl.
+  assert (match k v with | @Bind _ _ A0 e f => Bind e f | Return a =>  Return a | NoOp p' => NoOp p' end = k v) by (destruct (k v); easy).
+  rewrite H1. clear H1.
+  eapply weakenSafe. exact H.
+  apply H0.
+}
+(* {
+  rewrite frobProgId at 1. simpl.
+  econstructor. exact H. exact H1. easy.
+  intros.
+  specialize (H3 v).
+  split. easy.
+  destruct_all.
+  eapply lemBind.
+  exact H4.
+  exact H0.
+} *)
+apply undef.
+{
+}
+apply undef.
+Qed.
 
 Lemma weakenPost {A P Q Q'} {C : Prog E A} :
   VerifyProg i R G P C Q ->
@@ -85,10 +102,6 @@ Lemma weakenPrec {A P P' Q} {C : Prog E A} :
   VerifyProg i R G P C Q ->
   P' ==> P ->
   VerifyProg i R G P' C Q.
-Admitted.
-
-Lemma unfoldWhile {x : Prog E bool} {C : Prog E unit} :
-  while x C = (t <- x; if t then _ <- C; NoOp (while x C) else ret tt).
 Admitted.
 
 Lemma lemWhile {P} {T : Post VE VF bool} {Q : Post VE VF unit} {t : Prog E bool} {C : Prog E unit} :
@@ -127,4 +140,3 @@ easy.
 Qed.
 
 End rules.
-Set Guard Checking. *)
